proof/refine/RISCV64/ArchInvsDefs_H.thy
@@ -188,5 +188,17 @@ definition archMakeObjectT :: "arch_kernel_object_type \<Rightarrow> kernel_obje
      of PTET \<Rightarrow> injectKO (makeObject :: pte)
       | ASIDPoolT \<Rightarrow> injectKO (makeObject :: asidpool)"
 
+(* FIXME arch-split RT: split and probably move, it doesn't belong here but is used in Invariants_H *)
+lemma valid_sz_simps:
+  "objBitsKO ko < word_bits =
+    (case ko of
+      KOSchedContext sc \<Rightarrow> minSchedContextBits + scSize sc < word_bits
+    | _ \<Rightarrow>    True)"
+  by (cases ko;
+      clarsimp simp: objBits_def objBitsKO_def word_size_def archObjSize_def pageBits_def word_bits_def
+                     tcbBlockSizeBits_def epSizeBits_def ntfnSizeBits_def cteSizeBits_def word_size
+                     pteBits_def wordSizeCase_def wordBits_def replySizeBits_def
+              split: arch_kernel_object.splits)
+
 end
 end
