proof/refine/RISCV64/ArchInvsLemmas_H.thy
@@ -25,7 +25,8 @@ lemmas wordRadix_def' = wordRadix_def[simplified]
 lemma wordSizeCase_simp[simp]: "wordSizeCase a b = b"
   by (simp add: wordSizeCase_def wordBits_def word_size)
 
-lemmas objBits_defs = tcbBlockSizeBits_def epSizeBits_def ntfnSizeBits_def cteSizeBits_def
+lemmas objBits_defs =
+  tcbBlockSizeBits_def epSizeBits_def ntfnSizeBits_def cteSizeBits_def replySizeBits_def
 lemmas untypedBits_defs = minUntypedSizeBits_def maxUntypedSizeBits_def
 lemmas objBits_simps = objBits_def objBitsKO_def word_size_def archObjSize_def
 lemmas objBits_simps' = objBits_simps objBits_defs
@@ -107,9 +108,9 @@ named_theorems Invariants_H_cte_ats_assms
 (* FIXME arch-split: for proofs which require exact offsets lining up instead of cteSizeBits *)
 lemma raw_tcb_cte_cases_simps:
   "tcb_cte_cases 32 = Some (tcbVTable, tcbVTable_update)"
-  "tcb_cte_cases 64 = Some (tcbReply, tcbReply_update)"
-  "tcb_cte_cases 96 = Some (tcbCaller, tcbCaller_update)"
-  "tcb_cte_cases 128 = Some (tcbIPCBufferFrame, tcbIPCBufferFrame_update)"
+  "tcb_cte_cases 64 = Some (tcbIPCBufferFrame, tcbIPCBufferFrame_update)"
+  "tcb_cte_cases 96 = Some (tcbFaultHandler, tcbFaultHandler_update)"
+  "tcb_cte_cases 128 = Some (tcbTimeoutHandler, tcbTimeoutHandler_update)"
   by (simp add: tcb_cte_cases_def cteSizeBits_def)+
 
 lemma cte_wp_at_cases'[Invariants_H_cte_ats_assms]:
@@ -119,6 +120,7 @@ lemma cte_wp_at_cases'[Invariants_H_cte_ats_assms]:
    (\<exists>n tcb getF setF. ksPSpace s (p - n) = Some (KOTCB tcb) \<and> is_aligned (p - n) tcbBlockSizeBits
              \<and> tcb_cte_cases n = Some (getF, setF) \<and> P (getF tcb) \<and> ps_clear (p - n) tcbBlockSizeBits s))"
   (is "?LHS = ?RHS")
+  supply raw_tcb_cte_cases_simps[simp]
   apply (rule iffI)
    apply (clarsimp simp: cte_wp_at'_def gets_the_def readObject_def
                          getObject_def bind_def simpler_gets_def omonad_defs
@@ -324,10 +326,6 @@ lemma invs_pspace_in_kernel_mappings'[elim!]:
   "invs' s \<Longrightarrow> pspace_in_kernel_mappings' s"
   by (fastforce dest!: invs_valid_pspace' simp: valid_pspace'_def)
 
-lemma valid_pspace_in_kernel_mappings'[elim!]:
-  "valid_pspace' s \<Longrightarrow> pspace_in_kernel_mappings' s"
-  by (clarsimp simp: valid_pspace'_def)
-
 lemma tcb_hyp_refs_of'_simps[simp]:
   "tcb_hyp_refs' atcb = {}"
   by (auto simp: tcb_hyp_refs'_def)
@@ -347,34 +345,102 @@ lemma hyp_refs_of_live':
 lemmas valid_cap_simps' =
   valid_cap'_def[split_simps capability.split arch_capability.split]
 
-lemma is_physical_cases:
- "(capClass cap = PhysicalClass) =
-  (case cap of NullCap                         \<Rightarrow> False
-             | DomainCap                       \<Rightarrow> False
-             | IRQControlCap                   \<Rightarrow> False
-             | IRQHandlerCap irq               \<Rightarrow> False
-             | ReplyCap r m cr                 \<Rightarrow> False
-             | ArchObjectCap ASIDControlCap    \<Rightarrow> False
-             | _                               \<Rightarrow> True)"
-  by (simp split: capability.splits arch_capability.splits zombie_type.splits)
 
+(* FIXME arch-split RT: whole typ_at_lift section needs to be split *)
 lemma typ_at_lift_page_table_at'_strong:
-  "(\<And>P p. f \<lbrace>\<lambda>s. P (typ_at' (ArchT PTET) p s)\<rbrace>) \<Longrightarrow> f \<lbrace>\<lambda>s. P (page_table_at' p s)\<rbrace>"
-  unfolding page_table_at'_def All_less_Ball
-  apply (rule P_bool_lift[where P=P])
+  "(\<And>p. f \<lbrace>\<lambda>s. P (typ_at' (ArchT PTET) p s)\<rbrace>) \<Longrightarrow> f \<lbrace>\<lambda>s. P (page_table_at' p s)\<rbrace>"
+  unfolding page_table_at'_def
+  apply (rule bool_to_bool_cases[where f=P]; clarsimp)
   apply (wpsimp wp: hoare_vcg_const_Ball_lift hoare_vcg_bex_lift hoare_vcg_imp_lift
                     hoare_vcg_all_lift hoare_vcg_ex_lift
-         | fastforce)+
+         | assumption)+
   done
 
 lemma typ_at_lift_frame_at'_strong:
-  assumes "\<And>P T p. f \<lbrace>\<lambda>s. P (typ_at' T p s)\<rbrace>"
-  shows "f \<lbrace>\<lambda>s. P (frame_at' p sz d s)\<rbrace>"
+  "\<lbrakk>\<And>T p. f \<lbrace>\<lambda>s. P (typ_at' T p s)\<rbrace>\<rbrakk> \<Longrightarrow> f \<lbrace>\<lambda>s. P (frame_at' p sz d s)\<rbrace>"
+  supply if_split[split del]
   unfolding frame_at'_def
-  apply (rule P_bool_lift[where P=P])
-   apply (wpsimp wp: hoare_vcg_all_lift hoare_vcg_const_imp_lift assms hoare_vcg_ex_lift
-          split_del: if_split)+
+  apply (rule bool_to_bool_cases[where f=P]; clarsimp)
+   apply (wpsimp wp: hoare_vcg_all_lift hoare_vcg_const_imp_lift  hoare_vcg_ex_lift
+          | assumption)+
   done
+
+lemma valid_arch_tcb_lift'_strong:
+  assumes "\<And>T p. f \<lbrace>\<lambda>s. P (typ_at' T p s)\<rbrace>"
+  shows "f \<lbrace>\<lambda>s. P (valid_arch_tcb' tcb s)\<rbrace>"
+  by (clarsimp simp: valid_arch_tcb'_def, wp)
+
+(* FIXME arch-split RT: I think this is true for all architectures, if it isn't then
+                        typ_at'_valid_obj'_lift will need to be moved later, out of typ_at_lifts. *)
+lemma valid_arch_obj_lift'_strong:
+  assumes "\<And>T p. f \<lbrace>\<lambda>s. P (typ_at' T p s)\<rbrace>"
+  shows "f \<lbrace>\<lambda>s. P (valid_arch_obj' ako s)\<rbrace>"
+  by (clarsimp simp: valid_arch_obj'_def, wp)
+
+lemmas typ_at_lifts_strong =
+  typ_at_lift_tcb'_strong typ_at_lift_ep'_strong
+  typ_at_lift_ntfn'_strong typ_at_lift_cte'_strong
+  typ_at_lift_reply'_strong typ_at_lift_sc'_strong
+  typ_at_lift_valid_tcb_state'_strong
+  typ_at_lift_page_table_at'_strong
+  typ_at_lift_frame_at'_strong
+  valid_arch_tcb_lift'_strong
+  valid_arch_obj_lift'_strong
+
+lemma typ_at_lift_valid_irq_node':
+  assumes P: "\<And>P T p. \<lbrace>\<lambda>s. P (typ_at' T p s)\<rbrace> f \<lbrace>\<lambda>rv s. P (typ_at' T p s)\<rbrace>"
+  shows      "\<lbrace>valid_irq_node' p\<rbrace> f \<lbrace>\<lambda>_. valid_irq_node' p\<rbrace>"
+  apply (simp add: valid_irq_node'_def)
+  apply (wp hoare_vcg_all_lift P typ_at_lifts_strong)
+  done
+
+context begin
+\<comment>\<open> We're using @{command ML_goal} here because there are two useful formulations
+    of typ_at lifting lemmas and we do not want to write all of the possibilities
+    out by hand. If we use typ_at_lift_tcb' as an example, then the first is
+    @{term "\<lbrace>\<lambda>s. P (typ_at' TCBT p s)\<rbrace> f \<lbrace>\<lambda>_ s. P (typ_at' TCBT p s)\<rbrace>
+            \<Longrightarrow> \<lbrace>\<lambda>s. P (tcb_at' p s)\<rbrace> f \<lbrace>\<lambda>_ s. P (tcb_at' p s)\<rbrace>"} and the second is
+    @{term "(\<And>P. \<lbrace>\<lambda>s. P (typ_at' TCBT p s)\<rbrace> f \<lbrace>\<lambda>_ s. P (typ_at' TCBT p s)\<rbrace>)
+            \<Longrightarrow> \<lbrace>\<lambda>s. P (tcb_at' p s)\<rbrace> f \<lbrace>\<lambda>_ s. P (tcb_at' p s)\<rbrace>"}.
+    The first form is stronger, and therefore preferred for backward reasoning
+    using rule. However, since the P in the premise is free in the first form,
+    forward unification using the OF attribute produces flex-flex pairs which
+    causes problems. The second form avoids the unification issue by demanding
+    that there is a P that is free in the lemma supplied to the OF attribute.
+    However, it can only be applied if @{term f} preserves both
+    @{term "typ_at' TCBT p s"} and @{term "\<not> typ_at' TCBT p s"}.
+    The following @{command ML_goal} generates lemmas of the second form based on
+    the previously proven stronger lemmas of the first form. \<close>
+ML \<open>
+local
+  val strong_thms = @{thms typ_at_lifts_strong[no_vars]};
+  fun abstract_P term = Logic.all (Free ("P", @{typ "bool \<Rightarrow> bool"})) term
+  fun abstract thm =
+    let
+      val prems = List.map abstract_P (Thm.prems_of thm);
+      fun imp [] = Thm.concl_of thm
+        | imp (p :: pms) = @{const Pure.imp} $ p $ imp pms
+    in
+      imp prems
+    end
+in
+  val typ_at_lifts_internal_goals = List.map abstract strong_thms
+end
+\<close>
+
+private ML_goal typ_at_lifts_internal:
+  \<open>typ_at_lifts_internal_goals\<close>
+  by (auto simp: typ_at_lifts_strong)
+
+lemmas typ_at_lifts = typ_at_lifts_internal
+                      typ_at_lift_cte_at'
+                      valid_bound_tcb_lift
+                      valid_bound_reply_lift
+                      valid_bound_sc_lift
+                      valid_bound_ntfn_lift
+                      valid_ntfn_lift'
+                      valid_sc_lift'
+end
 
 lemma typ_at_lift_valid_cap':
   assumes P: "\<And>P T p. \<lbrace>\<lambda>s. P (typ_at' T p s)\<rbrace> f \<lbrace>\<lambda>rv s. P (typ_at' T p s)\<rbrace>"
@@ -401,16 +467,87 @@ lemma typ_at_lift_valid_cap':
                  hoare_vcg_all_lift typ_at_lifts_strong)+
   done
 
-(* interface lemma *)
-lemma valid_arch_tcb_lift':
-  assumes x: "\<And>T p. \<lbrace>typ_at' T p\<rbrace> f \<lbrace>\<lambda>rv. typ_at' T p\<rbrace>"
-  shows "\<lbrace>\<lambda>s. valid_arch_tcb' tcb s\<rbrace> f \<lbrace>\<lambda>rv s. valid_arch_tcb' tcb s\<rbrace>"
-  by (clarsimp simp add: valid_arch_tcb'_def, wp)
+lemma typ_at'_valid_obj'_lift:
+  assumes P: "\<And>P T p. \<lbrace>\<lambda>s. P (typ_at' T p s)\<rbrace> f \<lbrace>\<lambda>rv s. P (typ_at' T p s)\<rbrace>"
+  assumes sz: "\<And>n p. \<lbrace>\<lambda>s. sc_at'_n n p s\<rbrace> f \<lbrace>\<lambda>rv s. sc_at'_n n p s\<rbrace>"
+  notes [wp] = hoare_vcg_all_lift hoare_vcg_imp_lift' hoare_vcg_const_Ball_lift
+               typ_at_lifts[OF P] typ_at_lift_valid_cap'[OF P]
+  shows      "\<lbrace>\<lambda>s. valid_obj' obj s\<rbrace> f \<lbrace>\<lambda>rv s. valid_obj' obj s\<rbrace>"
+  supply raw_tcb_cte_cases_simps[simp] (* FIXME arch-split: legacy, try use tcb_cte_cases_neqs *)
+  apply (cases obj; simp add: valid_obj'_def hoare_TrueI)
+        apply (rename_tac endpoint)
+        apply (case_tac endpoint; simp add: valid_ep'_def, wp)
+       apply (rename_tac notification)
+       apply (case_tac "ntfnObj notification";
+               simp add: valid_ntfn'_def split: option.splits;
+               (wpsimp|rule conjI)+)
+      apply (rename_tac tcb)
+      apply (case_tac "tcbState tcb";
+             simp add: valid_tcb'_def valid_tcb_state'_def split_def opt_tcb_at'_def;
+             wpsimp wp: sz hoare_case_option_wp)
+     apply (wpsimp simp: valid_cte'_def sz)
+    apply (rename_tac arch_kernel_object)
+    apply (case_tac arch_kernel_object; wpsimp wp: sz)
+   apply wpsimp
+  apply (wpsimp simp: valid_reply'_def)
+  done
 
-lemmas typ_at_lifts =
-           typ_at_lift_tcb' typ_at_lift_ep' typ_at_lift_ntfn' typ_at_lift_cte' typ_at_lift_cte_at'
-           typ_at_lift_valid_untyped' typ_at_lift_valid_cap' valid_bound_tcb_lift
-           typ_at_lift_page_table_at' typ_at_lift_asid_at'
+lemma typ_at'_valid_sched_context'_lift:
+  assumes P: "\<And>P T p. \<lbrace>\<lambda>s. P (typ_at' T p s)\<rbrace> f \<lbrace>\<lambda>rv s. P (typ_at' T p s)\<rbrace>"
+  assumes sz: "\<And>n p. \<lbrace>\<lambda>s. sc_at'_n n p s\<rbrace> f \<lbrace>\<lambda>rv s. sc_at'_n n p s\<rbrace>"
+  notes [wp] = hoare_vcg_all_lift hoare_vcg_imp_lift' hoare_vcg_const_Ball_lift
+               typ_at_lifts[OF P] typ_at_lift_valid_cap'[OF P]
+  shows      "\<lbrace>\<lambda>s. valid_sched_context' ko s\<rbrace> f \<lbrace>\<lambda>rv s. valid_sched_context' ko s\<rbrace>"
+  by (wpsimp simp: valid_sched_context'_def)
+
+lemmas typ_at_sc_at'_n_lifts =
+  typ_at_lift_valid_untyped' typ_at_lift_valid_cap' typ_at'_valid_obj'_lift
+  typ_at'_valid_obj'_lift[where obj="KOEndpoint ko" for ko, simplified valid_obj'_def kernel_object.case]
+  typ_at'_valid_obj'_lift[where obj="KONotification ko" for ko, simplified valid_obj'_def kernel_object.case]
+  typ_at'_valid_obj'_lift[where obj="KOTCB ko" for ko, simplified valid_obj'_def kernel_object.case]
+  typ_at'_valid_obj'_lift[where obj="KOCTE ko" for ko, simplified valid_obj'_def kernel_object.case]
+  typ_at'_valid_obj'_lift[where obj="KOArch ko" for ko, simplified valid_obj'_def kernel_object.case]
+  typ_at'_valid_obj'_lift[where obj="KOReply ko" for ko, simplified valid_obj'_def kernel_object.case]
+  typ_at'_valid_sched_context'_lift
+
+lemmas typ_at_lifts_all = typ_at_lifts typ_at_sc_at'_n_lifts
+
+end
+
+locale typ_at_props' =
+  fixes f :: "'a kernel"
+  assumes typ': "f \<lbrace>\<lambda>s. P (typ_at' T p' s)\<rbrace>"
+begin
+
+interpretation Arch . (* FIXME arch-split RT *)
+
+lemmas typ_at_lifts'[wp] = typ_at_lifts[REPEAT [OF typ']]
+
+end
+
+locale typ_at_all_props' = typ_at_props' +
+  assumes scs: "f \<lbrace>\<lambda>s. Q (sc_at'_n n p s)\<rbrace>"
+begin
+
+interpretation Arch . (* FIXME arch-split RT *)
+
+lemmas typ_at_sc_at'_n_lifts'[wp] = typ_at_sc_at'_n_lifts[OF typ' scs]
+lemmas typ_at_lifts_all' = typ_at_lifts' typ_at_sc_at'_n_lifts'
+
+context begin
+(* We want to enforce that typ_at_lifts_all' only contains lemmas that have no
+   assumptions. The following thm statements should fail if this is not true. *)
+private lemmas check_valid_internal = iffD1[OF refl, where P="valid p g q" for p g q]
+thm typ_at_lifts_all'[atomized, THEN check_valid_internal]
+end
+
+end
+
+(* we expect typ_at' and sc_at'_n lemmas to be [wp], so this should be easy: *)
+method typ_at_props' = unfold_locales; wp?
+
+
+context Arch begin arch_global_naming
 
 lemma page_table_pte_atI':
   "page_table_at' p s \<Longrightarrow> pte_at' (p + (ucast (x::pt_index) << pte_bits)) s"
