proof/refine/RISCV64/CSpace_R.thy
@@ -3034,12 +3034,10 @@ crunch cteInsert
   (wp: crunch_wps)
 
 lemma cteInsert_vms'[wp]:
-  "\<lbrace>valid_machine_state'\<rbrace> cteInsert cap src dest \<lbrace>\<lambda>rv. valid_machine_state'\<rbrace>"
+  "cteInsert cap src dest \<lbrace>valid_machine_state'\<rbrace>"
   apply (simp add: cteInsert_def valid_machine_state'_def pointerInDeviceData_def
                    pointerInUserData_def)
-  apply (intro hoare_vcg_all_lift hoare_vcg_disj_lift)
-   apply (wp setObject_typ_at_inv setObject_ksMachine updateObject_default_inv |
-          intro hoare_drop_imp|assumption)+
+  apply (wpsimp wp: hoare_vcg_all_lift hoare_vcg_disj_lift hoare_drop_imps)
   done
 
 crunch cteInsert
